thys/Deep_Learning/DL_Rank_CP_Rank.thy
@@ -12,25 +12,25 @@ no_notation "normal_rel"  (infixl "\<lhd>" 60)
 
 lemma lookup_order1_prod:
 assumes "\<And>B. B\<in>set Bs \<Longrightarrow> Tensor.order B = 1" 
-assumes "is \<lhd> dims (listprod Bs)"
-shows "lookup (listprod Bs) is = listprod (map (\<lambda>(i,B). lookup B [i]) (zip is Bs))"
+assumes "is \<lhd> dims (prod_list Bs)"
+shows "lookup (prod_list Bs) is = prod_list (map (\<lambda>(i,B). lookup B [i]) (zip is Bs))"
 using assms proof (induction Bs arbitrary:"is")
   case Nil
-  then show ?case unfolding "listprod.Nil" unfolding zip.simps tensor_one_def 
-    by (metis (no_types, lifting) dims_tensor_from_lookup length_greater_0_conv length_map listprod.Nil 
+  then show ?case unfolding "prod_list.Nil" unfolding zip.simps tensor_one_def 
+    by (metis (no_types, lifting) dims_tensor_from_lookup length_greater_0_conv length_map prod_list.Nil 
     lookup_tensor_from_lookup tensor_one_def tensor_one_from_lookup)
 next
   case (Cons B Bs "is'")
   then obtain i "is" where "is' = i # is" 
-    by (metis append_is_Nil_conv dims_tensor_prod length_0_conv list.set_intros(1) listprod.Cons valid_index.simps zero_neq_one)
+    by (metis append_is_Nil_conv dims_tensor_prod length_0_conv list.set_intros(1) prod_list.Cons valid_index.simps zero_neq_one)
   have "Tensor.order B = 1" using Cons by auto
   then have valid1:"[i] \<lhd> dims B"
-    using `is' \<lhd> dims (listprod (B # Bs))`[unfolded listprod.Cons dims_tensor_prod `is' = i # is`] 
+    using `is' \<lhd> dims (prod_list (B # Bs))`[unfolded prod_list.Cons dims_tensor_prod `is' = i # is`] 
     by (metis One_nat_def Suc_length_conv hd_append2 length_0_conv list.sel(1) list.simps(3) valid_index.Nil valid_index.simps)
-  have valid2:"is \<lhd> dims (listprod Bs)" 
-    using `is' \<lhd> dims (listprod (B # Bs))`[unfolded listprod.Cons dims_tensor_prod `is' = i # is`] `Tensor.order B = 1`
+  have valid2:"is \<lhd> dims (prod_list Bs)" 
+    using `is' \<lhd> dims (prod_list (B # Bs))`[unfolded prod_list.Cons dims_tensor_prod `is' = i # is`] `Tensor.order B = 1`
     by (metis One_nat_def Suc_length_conv append_eq_Cons_conv length_0_conv list.sel(3) list.simps(3) self_append_conv2 valid_indexE)
-  show ?case unfolding `is' = i # is` List.zip_Cons_Cons List.list.map(2) listprod.Cons 
+  show ?case unfolding `is' = i # is` List.zip_Cons_Cons List.list.map(2) prod_list.Cons 
     lookup_tensor_prod[OF valid1 valid2, simplified] by (simp add: Cons.IH Cons.prems(1) valid2)
 qed
 
@@ -39,19 +39,19 @@ fixes A::"'a::field tensor"
 assumes "cprank_max1 A"
 shows "mrank (matricize I A) \<le> 1" 
 proof -
-  obtain Bs a where "\<And>B. B \<in> set Bs \<Longrightarrow> Tensor.order B = 1" "a \<cdot> listprod Bs = A"
-    using cprank_max1_listprodE assms by metis
-  def row_factor == "\<lambda>ris. a * (listprod (map (\<lambda>(i,B). lookup B [i]) (zip ris (sublist Bs I))))"
-  def col_factor == "\<lambda>cis. (listprod (map (\<lambda>(i,B). lookup B [i]) (zip cis (sublist Bs (-I)))))"
+  obtain Bs a where "\<And>B. B \<in> set Bs \<Longrightarrow> Tensor.order B = 1" "a \<cdot> prod_list Bs = A"
+    using cprank_max1_prod_listE assms by metis
+  def row_factor == "\<lambda>ris. a * (prod_list (map (\<lambda>(i,B). lookup B [i]) (zip ris (sublist Bs I))))"
+  def col_factor == "\<lambda>cis. (prod_list (map (\<lambda>(i,B). lookup B [i]) (zip cis (sublist Bs (-I)))))"
   have "\<And>is. is \<lhd> dims A \<Longrightarrow> lookup A is = row_factor (sublist is I) * col_factor (sublist is (-I))"
   proof -
     fix "is" assume "is \<lhd> dims A"
-    then have "lookup A is = a * (listprod (map (\<lambda>(i,B). lookup B [i]) (zip is Bs)))" 
+    then have "lookup A is = a * (prod_list (map (\<lambda>(i,B). lookup B [i]) (zip is Bs)))" 
       using lookup_order1_prod[OF `\<And>B. B \<in> set Bs \<Longrightarrow> Tensor.order B = 1`] lookup_smult 
-      using \<open>a \<cdot> listprod Bs = A\<close> dims_smult by fastforce
-    also have "... = a * (listprod (map (\<lambda>(i,B). lookup B [i]) (sublist (zip is Bs) I))) * 
-                         (listprod (map (\<lambda>(i,B). lookup B [i]) (sublist (zip is Bs) (-I))))"
-      using listprod_complementary_sublists by auto
+      using \<open>a \<cdot> prod_list Bs = A\<close> dims_smult by fastforce
+    also have "... = a * (prod_list (map (\<lambda>(i,B). lookup B [i]) (sublist (zip is Bs) I))) * 
+                         (prod_list (map (\<lambda>(i,B). lookup B [i]) (sublist (zip is Bs) (-I))))"
+      using prod_list_complementary_sublists by auto
     also have "... = row_factor (sublist is I) * col_factor (sublist is (-I))"
       using sublist_zip row_factor_def col_factor_def by metis
     finally show "lookup A is = row_factor (sublist is I) * col_factor (sublist is (-I))" .
